Foundation/Modal/Kripke/Logic/K.lean
@@ -8,21 +8,29 @@ open Kripke
 open Hilbert.Kripke
 
 
+namespace Kripke
+
+@[reducible] protected alias FrameClass.K := FrameClass.all
+@[reducible] protected alias FrameClass.finite_K := FrameClass.finite_all
+
+end Kripke
+
+
 namespace Hilbert.K.Kripke
 
-instance : Sound (Hilbert.K) FrameClass.all := instSound_of_validates_axioms FrameClass.all.validates_axiomK
+instance : Sound (Hilbert.K) FrameClass.K := instSound_of_validates_axioms FrameClass.all.validates_axiomK
 
-instance : Sound (Hilbert.K) FrameClass.finite_all := instSound_of_validates_axioms FrameClass.finite_all.validates_axiomK
+instance : Sound (Hilbert.K) FrameClass.finite_K := instSound_of_validates_axioms FrameClass.finite_all.validates_axiomK
 
-instance : Entailment.Consistent (Hilbert.K) := consistent_of_sound_frameclass FrameClass.all (by simp)
+instance : Entailment.Consistent (Hilbert.K) := consistent_of_sound_frameclass FrameClass.K (by simp)
 
-instance : Kripke.Canonical (Hilbert.K) FrameClass.all := ⟨by trivial⟩
+instance : Kripke.Canonical (Hilbert.K) FrameClass.K := ⟨by trivial⟩
 
-instance : Complete (Hilbert.K) FrameClass.all := inferInstance
+instance : Complete (Hilbert.K) FrameClass.K := inferInstance
 
-instance : Complete (Hilbert.K) (FrameClass.finite_all) := ⟨by
+instance : Complete (Hilbert.K) (FrameClass.finite_K) := ⟨by
   intro φ hp;
-  apply Complete.complete (𝓜 := FrameClass.all);
+  apply Complete.complete (𝓜 := FrameClass.K);
   intro F _ V x;
   let M : Kripke.Model := ⟨F, V⟩;
   let FM := coarsestFiltrationModel M ↑φ.subformulas;
@@ -36,7 +44,7 @@ instance : Complete (Hilbert.K) (FrameClass.finite_all) := ⟨by
 end Hilbert.K.Kripke
 
 
-lemma K.Kripke.eq_all : Modal.K = FrameClass.all.logic := eq_hilbert_logic_frameClass_logic
-lemma K.Kripke.eq_finite_all : Modal.K = FrameClass.finite_all.logic := eq_hilbert_logic_frameClass_logic
+lemma K.Kripke.eq_K : Modal.K = FrameClass.K.logic := eq_hilbert_logic_frameClass_logic
+lemma K.Kripke.eq_finite_K : Modal.K = FrameClass.finite_K.logic := eq_hilbert_logic_frameClass_logic
 
 end LO.Modal
