Foundation/Modal/Kripke/Logic/KD4Point3Z.lean
@@ -16,7 +16,7 @@ open Hilbert.Kripke
 
 namespace Logic.KD4Point3Z.Kripke
 
-instance sound_natLT : Sound Hilbert.KD4Point3Z natLT := instSound_of_frame_validates_axioms $ by
+instance : Sound Hilbert.KD4Point3Z natLT := instSound_of_frame_validates_axioms $ by
   simp only [Semantics.RealizeSet.insert_iff, ValidOnFrame.models_iff, Semantics.RealizeSet.singleton_iff];
   refine ⟨?_, ?_, ?_, ?_, ?_⟩;
   . apply FrameClass.all.validates_axiomK <;> tauto;
